theories/typing/type.v
@@ -35,20 +35,21 @@ Section type.
          invariants, which does not need the mask.  Moreover, it is
          more consistent with thread-local tokens, which we do not
          give any. *)
-      ty_share E N κ l tid : mgmtE ⊥ ↑N → mgmtE ⊆ E →
-        lft_ctx -∗ &{κ} (l ↦∗: ty_own tid) ={E}=∗ ty_shr κ tid (↑N) l;
+      ty_share E N κ l tid q : mgmtE ⊥ ↑N → mgmtE ⊆ E →
+        lft_ctx -∗ &{κ} (l ↦∗: ty_own tid) -∗ q.[κ] ={E}=∗
+        ty_shr κ tid (↑N) l ∗ q.[κ];
       ty_shr_mono κ κ' tid E E' l : E ⊆ E' →
         lft_ctx -∗ κ' ⊑ κ -∗ ty_shr κ tid E l -∗ ty_shr κ' tid E' l
     }.
   Global Existing Instances ty_shr_persistent.
 
-  Class Copy (ty : type) := {
-    copy_persistent tid vl : PersistentP (ty.(ty_own) tid vl);
+  Class Copy (t : type) := {
+    copy_persistent tid vl : PersistentP (t.(ty_own) tid vl);
     copy_shr_acc κ tid E F l q :
       mgmtE ∪ F ⊆ E →
-      lft_ctx -∗ ty.(ty_shr) κ tid F l -∗
-        q.[κ] ∗ na_own tid F ={E}=∗ ∃ q', ▷l ↦∗{q'}: ty.(ty_own) tid ∗
-          (▷l ↦∗{q'}: ty.(ty_own) tid ={E}=∗ q.[κ] ∗ na_own tid F)
+      lft_ctx -∗ t.(ty_shr) κ tid F l -∗
+        q.[κ] ∗ na_own tid F ={E}=∗ ∃ q', ▷l ↦∗{q'}: t.(ty_own) tid ∗
+          (▷l ↦∗{q'}: t.(ty_own) tid ={E}=∗ q.[κ] ∗ na_own tid F)
   }.
   Global Existing Instances copy_persistent.
 
@@ -76,42 +77,38 @@ Section type.
           [subtype_shr_mono]. *)
        ty_shr := λ κ tid _ l,
                  (∃ vl, (&frac{κ} λ q, l ↦∗{q} vl) ∗
-                        (▷ st.(st_own) tid vl ∨ □|={↑lftN}=>[†κ]))%I
+                        ▷ st.(st_own) tid vl)%I
     |}.
   Next Obligation. intros. apply st_size_eq. Qed.
   Next Obligation.
-    intros st E N κ l tid ? ?. iIntros "#LFT Hmt".
+    intros st E N κ l tid ? ? ?. iIntros "#LFT Hmt Hκ".
     iMod (bor_exists with "LFT Hmt") as (vl) "Hmt". set_solver.
     iMod (bor_sep with "LFT Hmt") as "[Hmt Hown]". set_solver.
     iMod (bor_persistent with "LFT Hown") as "[Hown|#H†]". set_solver.
-    - iMod (bor_fracture with "LFT [Hmt]") as "Hfrac"; last first.
+    - iFrame "Hκ". iMod (bor_fracture with "LFT [Hmt]") as "Hfrac"; last first.
       { iExists vl. iFrame. auto. }
       done. set_solver.
-    - iExists []. iSplitL; last by auto. iApply (frac_bor_fake with "LFT"); auto.
+    - iExFalso. iApply (lft_tok_dead with "Hκ"). done.
   Qed.
   Next Obligation.
     intros st κ κ' tid E E' l ?. iIntros "#LFT #Hord H".
     iDestruct "H" as (vl) "[#Hf #Hown]".
-    iExists vl. iSplit. by iApply (frac_bor_shorten with "Hord").
-    iDestruct "Hown" as "[Hown|#H†]". auto. iRight. iIntros "!#".
-    by iApply (lft_incl_dead with "Hord >").
+    iExists vl. iFrame "Hown". by iApply (frac_bor_shorten with "Hord").
   Qed.
 
   Global Program Instance ty_of_st_copy st : Copy (ty_of_st st).
   Next Obligation.
     intros st κ tid E F l q ?. iIntros "#LFT #Hshr[Hlft $]".
-    iDestruct "Hshr" as (vl) "[Hf [Hown|#H†]]".
-    - iMod (frac_bor_acc with "LFT Hf Hlft") as (q') "[Hmt Hclose]"; first set_solver.
-      iModIntro. iExists _. iDestruct "Hmt" as "[Hmt1 Hmt2]". iSplitL "Hmt1".
-      + iNext. iExists _. by iFrame.
-      + iIntros "Hmt1". iDestruct "Hmt1" as (vl') "[Hmt1 #Hown']".
-        iAssert (▷ ⌜length vl = length vl'⌝)%I as ">%".
-        { iNext. iDestruct (st_size_eq with "Hown") as %->.
-          iDestruct (st_size_eq with "Hown'") as %->. done. }
-        iCombine "Hmt1" "Hmt2" as "Hmt". rewrite heap_mapsto_vec_op // Qp_div_2.
-        iDestruct "Hmt" as "[>% Hmt]". subst. by iApply "Hclose".
-    - iApply fupd_mask_mono; last iMod "H†". set_solver.
-      iDestruct (lft_tok_dead with "Hlft H†") as "[]".
+    iDestruct "Hshr" as (vl) "[Hf Hown]".
+    iMod (frac_bor_acc with "LFT Hf Hlft") as (q') "[Hmt Hclose]"; first set_solver.
+    iModIntro. iExists _. iDestruct "Hmt" as "[Hmt1 Hmt2]". iSplitL "Hmt1".
+    - iNext. iExists _. by iFrame.
+    - iIntros "Hmt1". iDestruct "Hmt1" as (vl') "[Hmt1 #Hown']".
+      iAssert (▷ ⌜length vl = length vl'⌝)%I as ">%".
+      { iNext. iDestruct (st_size_eq with "Hown") as %->.
+        iDestruct (st_size_eq with "Hown'") as %->. done. }
+      iCombine "Hmt1" "Hmt2" as "Hmt". rewrite heap_mapsto_vec_op // Qp_div_2.
+      iDestruct "Hmt" as "[>% Hmt]". subst. by iApply "Hclose".
   Qed.
 End type.
 
@@ -180,7 +177,7 @@ Section subtyping.
     intros Hst. iIntros. iSplit; first done. iSplit; iAlways.
     - iIntros. iApply (Hst with "* [] [] []"); done.
     - iIntros (????) "H".
-      iDestruct "H" as (vl) "[Hf [Hown|H†]]"; iExists vl; iFrame "Hf"; last by auto.
-      iLeft. by iApply (Hst with "* [] [] []").
+      iDestruct "H" as (vl) "[Hf Hown]". iExists vl. iFrame "Hf".
+      by iApply (Hst with "* [] [] []").
   Qed.
 End subtyping.
