theories/typing/product.v
@@ -9,7 +9,7 @@ Section product.
   Program Definition unit : type :=
     {| ty_size := 0; ty_own tid vl := ⌜vl = []⌝%I; ty_shr κ tid E l := True%I |}.
   Next Obligation. iIntros (tid vl) "%". by subst. Qed.
-  Next Obligation. by iIntros (???????) "_ _". Qed.
+  Next Obligation. by iIntros (????????) "_ _ $". Qed.
   Next Obligation. by iIntros (???????) "_ _ $". Qed.
 
   Global Instance unit_copy : Copy unit.
@@ -49,11 +49,11 @@ Section product.
     iDestruct "H1" as %->. iDestruct "H2" as %->. done.
   Qed.
   Next Obligation.
-    intros ty1 ty2 E N κ l tid ??. iIntros "#LFT /=H". rewrite split_prod_mt.
+    intros ty1 ty2 E N κ l tid q ??. iIntros "#LFT /=H Htok". rewrite split_prod_mt.
     iMod (bor_sep with "LFT H") as "[H1 H2]". set_solver.
-    iMod (ty1.(ty_share) _ (N .@ 1) with "LFT H1") as "?". solve_ndisj. done.
-    iMod (ty2.(ty_share) _ (N .@ 2) with "LFT H2") as "?". solve_ndisj. done.
-    iModIntro. iExists (↑N .@ 1). iExists (↑N .@ 2). iFrame.
+    iMod (ty1.(ty_share) _ (N .@ 1) with "LFT H1 Htok") as "[? Htok]". solve_ndisj. done.
+    iMod (ty2.(ty_share) _ (N .@ 2) with "LFT H2 Htok") as "[? Htok]". solve_ndisj. done.
+    iModIntro. iFrame "Htok". iExists (↑N .@ 1). iExists (↑N .@ 2). iFrame.
     iPureIntro. split. solve_ndisj. split; apply nclose_subseteq.
   Qed.
   Next Obligation.
