theories/typing/shr_bor.v
@@ -39,22 +39,28 @@ Section typing.
   Context `{typeG Σ}.
 
   Lemma tctx_incl_share E L p κ ty :
-    tctx_incl E L [TCtx_holds p (&uniq{κ}ty)] [TCtx_holds p (&shr{κ}ty)].
+    lctx_lft_alive E L κ → tctx_incl E L [TCtx_hasty p (&uniq{κ}ty)] [TCtx_hasty p (&shr{κ}ty)].
   Proof.
-    iIntros (?) "#LFT _ _ Huniq". rewrite /tctx_interp !big_sepL_singleton /=.
-    iDestruct "Huniq" as (v) "[% Huniq]". iExists _. iFrame "%".
+    iIntros (Hκ ???) "#LFT HE HL Huniq".
+    iMod (Hκ with "HE HL") as (q) "[Htok Hclose]"; [try done..|].
+    rewrite /tctx_interp !big_sepL_singleton /=.
+    iDestruct "Huniq" as (v) "[% Huniq]". 
     iDestruct "Huniq" as (l P) "[[% #HPiff] HP]".
     iMod (bor_iff with "LFT [] HP") as "H↦". set_solver. by eauto.
-    iMod (ty.(ty_share) _ lrustN with "LFT H↦") as "Hown"; [solve_ndisj|done|].
+    iMod (ty.(ty_share) _ lrustN with "LFT H↦ Htok") as "[Hown Htok]"; [solve_ndisj|done|].
+    iMod ("Hclose" with "Htok") as "[$ $]". iExists _. iFrame "%".
     iIntros "!>/=". eauto.
   Qed.
 
   Lemma tctx_reborrow_shr E L p ty κ κ' :
     lctx_lft_incl E L κ' κ →
-    tctx_incl E L [TCtx_holds p (&shr{κ}ty)]
-                  [TCtx_holds p (&shr{κ'}ty); TCtx_guarded p κ (&shr{κ}ty)].
+    tctx_incl E L [TCtx_hasty p (&shr{κ}ty)]
+                  [TCtx_hasty p (&shr{κ'}ty); TCtx_guarded p κ (&shr{κ}ty)].
   Proof.
-    iIntros (Hκκ' tid) "#LFT #HE #HL H". iDestruct (Hκκ' with "HE HL") as "Hκκ'".
+    iIntros (Hκκ' tid ??) "#LFT HE HL H".
+    iDestruct (elctx_interp_persist with "HE") as "#HE'".
+    iDestruct (llctx_interp_persist with "HL") as "#HL'". iFrame "HE HL".
+    iDestruct (Hκκ' with "HE' HL'") as "Hκκ'".
     rewrite /tctx_interp big_sepL_singleton big_sepL_cons big_sepL_singleton.
     iDestruct "H" as (v) "[% #H]". iDestruct "H" as (l) "[EQ Hshr]".
     iDestruct "EQ" as %[=->]. simpl. iModIntro. iSplit.
@@ -88,19 +94,18 @@ Section typing.
                (!ν)
                (λ v, v ◁ &shr{κ} ty ∗ κ' ⊑ κ ∗ q.[κ'])%P.
   Proof.
-    iIntros (tid) "!#(#HEAP & #LFT & (H◁ & #H⊑ & Htok) & $)". wp_bind ν.
+    iIntros (tid) "!#(#HEAP & #LFT & (H◁ & #H⊑ & [Htok1 Htok2]) & $)". wp_bind ν.
     iApply (has_type_wp with "H◁"). iIntros (v) "Hνv H◁!>". iDestruct "Hνv" as %Hνv.
     rewrite has_type_value. iDestruct "H◁" as (l) "[Heq #H↦]". iDestruct "Heq" as %[=->].
-    iMod (lft_incl_acc with "H⊑ Htok") as (q'') "[Htok Hclose]". done.
+    iMod (lft_incl_acc with "H⊑ Htok1") as (q'') "[Htok1 Hclose]". done.
     iDestruct "H↦" as (vl) "[H↦b #Hown]".
-    iMod (frac_bor_acc with "LFT H↦b Htok") as (q''') "[>H↦ Hclose']". done.
-    iApply (wp_fupd_step _ (⊤∖↑lrustN∖↑lftN) with "[Hown]"); try done.
-    - iApply ("Hown" with "* [%]"). set_solver.
-    - wp_read. iIntros "!>[Hshr|#H†]{$H⊑}".
-      + iSplitL "Hshr"; first by iExists _; auto. iApply ("Hclose" with ">").
-        iFrame. iApply "Hclose'". auto.
-      + iMod ("Hclose'" with "[H↦]"). by auto.
-        by iDestruct (lft_tok_dead with "[-] H†") as "[]".
+    iMod (frac_bor_acc with "LFT H↦b Htok1") as (q''') "[>H↦ Hclose']". done.
+    iMod (lft_incl_acc with "H⊑ Htok2") as (q2) "[Htok2 Hclose'']". solve_ndisj.
+    iApply (wp_fupd_step _ (⊤∖↑lrustN∖↑lftN) with "[Hown Htok2]"); try done.
+    - iApply ("Hown" with "* [%] Htok2"). set_solver.
+    - wp_read. iIntros "!>[Hshr Htok2]{$H⊑}". iMod ("Hclose''" with "Htok2") as "$".
+      iSplitL "Hshr"; first by iExists _; auto. iApply ("Hclose" with ">").
+      iFrame. iApply "Hclose'". auto.
   Qed.
 
   Lemma typed_deref_shr_bor_bor ty ν κ κ' κ'' q:
@@ -108,21 +113,21 @@ Section typing.
                (!ν)
                (λ v, v ◁ &shr{κ'} ty ∗ κ ⊑ κ' ∗ q.[κ])%P.
   Proof.
-    iIntros (tid) "!#(#HEAP & #LFT & (H◁ & #H⊑1 & Htok & #H⊑2) & $)". wp_bind ν.
+    iIntros (tid) "!#(#HEAP & #LFT & (H◁ & #H⊑1 & [Htok1 Htok2] & #H⊑2) & $)". wp_bind ν.
     iApply (has_type_wp with "H◁"). iIntros (v) "Hνv H◁!>". iDestruct "Hνv" as %Hνv.
     rewrite has_type_value. iDestruct "H◁" as (l) "[Heq Hshr]".
     iDestruct "Heq" as %[=->]. iDestruct "Hshr" as (l') "[H↦ Hown]".
-    iMod (lft_incl_acc with "H⊑1 Htok") as (q') "[Htok Hclose]". done.
-    iMod (frac_bor_acc with "LFT H↦ Htok") as (q'') "[>H↦ Hclose']". done.
+    iMod (lft_incl_acc with "H⊑1 Htok1") as (q') "[Htok1 Hclose]". done.
+    iMod (frac_bor_acc with "LFT H↦ Htok1") as (q'') "[>H↦ Hclose']". done.
     iAssert (κ' ⊑ κ'' ∪ κ')%I as "#H⊑3".
     { iApply (lft_incl_glb with "H⊑2 []"). iApply lft_incl_refl. }
-    iApply (wp_fupd_step _ (_∖_) with "[Hown]"); try done.
-    - iApply ("Hown" with "* [%]"). set_solver.
-    - wp_read. iIntros "!>[#Hshr|#H†]{$H⊑1}".
-      + iSplitR.
-        * iExists _. iSplitR. done. by iApply (ty_shr_mono with "LFT H⊑3 Hshr").
-        * iApply ("Hclose" with ">"). iApply ("Hclose'" with "[$H↦]").
-      + iMod ("Hclose'" with "[H↦]"). by auto.
-        by iDestruct (lft_tok_dead with "[-] H†") as "[]".
+    iMod (lft_incl_acc with "[] Htok2") as (q2) "[Htok2 Hclose'']". solve_ndisj.
+    { iApply (lft_incl_trans with "[]"); done. }
+    iApply (wp_fupd_step _ (_∖_) with "[Hown Htok2]"); try done.
+    - iApply ("Hown" with "* [%] Htok2"). set_solver.
+    - wp_read. iIntros "!>[#Hshr Htok2]{$H⊑1}".
+      iMod ("Hclose''" with "Htok2") as "$". iSplitR.
+      * iExists _. iSplitR. done. by iApply (ty_shr_mono with "LFT H⊑3 Hshr").
+      * iApply ("Hclose" with ">"). iApply ("Hclose'" with "[$H↦]").
   Qed.
 End typing.
