theories/typing/uniq_bor.v
@@ -16,36 +16,35 @@ Section uniq_bor.
          (∃ (l:loc) P, (⌜vl = [ #l ]⌝ ∗ □ (P ↔ l ↦∗: ty.(ty_own) tid)) ∗ &{κ} P)%I;
        ty_shr κ' tid E l :=
          (∃ l':loc, &frac{κ'}(λ q', l ↦{q'} #l') ∗
-            □ ∀ F, ⌜E ∪ mgmtE ⊆ F⌝
-                ={F, F∖E∖↑lftN}▷=∗ ty.(ty_shr) (κ∪κ') tid E l' ∨ [†κ'])%I
+            □ ∀ F q, ⌜E ∪ mgmtE ⊆ F⌝ -∗ q.[κ∪κ']
+                ={F, F∖E∖↑lftN}▷=∗ ty.(ty_shr) (κ∪κ') tid E l' ∗ q.[κ∪κ'])%I
     |}.
   Next Obligation.
     iIntros (q ty tid vl) "H". iDestruct "H" as (l P) "[[% _] _]". by subst.
   Qed.
   Next Obligation.
-    move=> κ ty E N κ' l tid ??/=. iIntros "#LFT Hshr".
+    move=> κ ty E N κ' l tid ???/=. iIntros "#LFT Hshr Htok".
     iMod (bor_exists with "LFT Hshr") as (vl) "Hb". set_solver.
     iMod (bor_sep with "LFT Hb") as "[Hb1 Hb2]". set_solver.
-    iMod (bor_exists with "LFT Hb2") as (l') "Hb2". set_solver. iExists l'.
+    iMod (bor_exists with "LFT Hb2") as (l') "Hb2". set_solver.
     iMod (bor_exists with "LFT Hb2") as (P) "Hb2". set_solver.
     iMod (bor_sep with "LFT Hb2") as "[H Hb2]". set_solver.
-    iMod (bor_persistent with "LFT H") as "[[>% #HPiff]|#H†]". set_solver.
-    - subst. rewrite heap_mapsto_vec_singleton.
-      iMod (bor_fracture (λ q, l ↦{q} #l')%I with "LFT Hb1") as "$". set_solver.
-      rewrite {1}bor_unfold_idx. iDestruct "Hb2" as (i) "[#Hpb Hpbown]".
-      iMod (inv_alloc N _ (idx_bor_own 1 i ∨ ty_shr ty (κ∪κ') tid (↑N) l')%I
-            with "[Hpbown]") as "#Hinv"; first by eauto.
-      iIntros "!>!#*%". iMod (inv_open with "Hinv") as "[INV Hclose]". set_solver.
-      iDestruct "INV" as "[>Hbtok|#Hshr]".
-      + iMod (bor_unnest _ _ _ P with "LFT [Hbtok]") as "Hb".
-        { set_solver. } { iApply bor_unfold_idx. eauto. }
-        iModIntro. iNext. iMod "Hb".
-        iMod (bor_iff with "LFT [] Hb") as "Hb". set_solver. by eauto.
-        iMod (ty.(ty_share) with "LFT Hb") as "#Hshr". done. set_solver.
-        iMod ("Hclose" with "[]") as "_"; auto.
-      + iMod ("Hclose" with "[]") as "_". by eauto.
-        iApply step_fupd_intro. set_solver. auto.
-    - iSplitL. by iApply (frac_bor_fake with "LFT"). iIntros "!>!#*_".
+    iMod (bor_persistent_tok with "LFT H Htok") as "[[>% #HPiff] Htok]". set_solver.
+    iFrame "Htok". iExists l'.
+    subst. rewrite heap_mapsto_vec_singleton.
+    iMod (bor_fracture (λ q, l ↦{q} #l')%I with "LFT Hb1") as "$". set_solver.
+    rewrite {1}bor_unfold_idx. iDestruct "Hb2" as (i) "[#Hpb Hpbown]".
+    iMod (inv_alloc N _ (idx_bor_own 1 i ∨ ty_shr ty (κ∪κ') tid (↑N) l')%I
+          with "[Hpbown]") as "#Hinv"; first by eauto.
+    iIntros "!> !# * % Htok". iMod (inv_open with "Hinv") as "[INV Hclose]". set_solver.
+    iDestruct "INV" as "[>Hbtok|#Hshr]".
+    - iMod (bor_unnest _ _ _ P with "LFT [Hbtok]") as "Hb".
+      { set_solver. } { iApply bor_unfold_idx. eauto. }
+                      iModIntro. iNext. iMod "Hb".
+      iMod (bor_iff with "LFT [] Hb") as "Hb". set_solver. by eauto.
+      iMod (ty.(ty_share) with "LFT Hb Htok") as "[#Hshr $]". done. set_solver.
+      iMod ("Hclose" with "[]") as "_"; auto.
+    - iMod ("Hclose" with "[]") as "_". by eauto.
       iApply step_fupd_intro. set_solver. auto.
   Qed.
   Next Obligation.
@@ -56,16 +55,16 @@ Section uniq_bor.
       - iApply (lft_incl_trans with "[] Hκ").
         iApply lft_le_incl. apply gmultiset_union_subseteq_r. }
     iExists l'. iSplit. by iApply (frac_bor_shorten with "[]").
-    iIntros "!#*%".
+    iIntros "!# * % Htok".
     iApply (step_fupd_mask_mono F _ _ (F∖E∖ ↑lftN)); try  set_solver.
-    iMod ("Hvs" with "* [%]") as "Hvs'". set_solver. iModIntro. iNext.
-    iMod "Hvs'" as "[#Hshr|H†]".
-    - iLeft. by iApply (ty_shr_mono with "LFT Hκ0").
-    - iRight. iApply (lft_incl_dead with "Hκ H†"). set_solver.
+    iMod (lft_incl_acc with "Hκ0 Htok") as (q') "[Htok Hclose]"; first set_solver.
+    iMod ("Hvs" with "* [%] Htok") as "Hvs'". set_solver. iModIntro. iNext.
+    iMod "Hvs'" as "[#Hshr Htok]". iMod ("Hclose" with "Htok") as "$".
+    by iApply (ty_shr_mono with "LFT Hκ0").
   Qed.
 
   Global Instance subtype_uniq_mono E L :
-    Proper (lctx_lft_incl E L --> eqtype E L ==> subtype E L) uniq_bor.
+    Proper (flip (lctx_lft_incl E L) ==> eqtype E L ==> subtype E L) uniq_bor.
   Proof.
     intros κ1 κ2 Hκ ty1 ty2 [Hty1 Hty2]. iIntros. iSplit; first done.
     iDestruct (Hty1 with "* [] [] []") as "(_ & #Ho1 & #Hs1)"; [done..|clear Hty1].
@@ -84,10 +83,11 @@ Section uniq_bor.
         - iApply (lft_incl_trans with "[] Hκ"). iApply lft_le_incl.
           apply gmultiset_union_subseteq_l.
         - iApply lft_le_incl. apply gmultiset_union_subseteq_r. }
-      iDestruct "H" as (l') "[Hbor #Hupd]". iExists l'. iIntros "{$Hbor}!#%%".
-      iMod ("Hupd" with "* [%]") as "Hupd'"; try done. iModIntro. iNext.
-      iMod "Hupd'" as "[H|H†]"; last by auto.
-      iLeft. iApply (ty_shr_mono with "[] Hincl'"); [done..|]. by iApply "Hs1".
+      iDestruct "H" as (l') "[Hbor #Hupd]". iExists l'. iIntros "{$Hbor}!# %%% Htok".
+      iMod (lft_incl_acc with "Hincl' Htok") as (q') "[Htok Hclose]"; first set_solver.
+      iMod ("Hupd" with "* [%] Htok") as "Hupd'"; try done. iModIntro. iNext.
+      iMod "Hupd'" as "[H Htok]". iMod ("Hclose" with "Htok") as "$".
+      iApply (ty_shr_mono with "[] Hincl'"); [done..|]. by iApply "Hs1".
   Qed.
   Global Instance subtype_uniq_mono' E L :
     Proper (lctx_lft_incl E L ==> eqtype E L ==> flip (subtype E L)) uniq_bor.
@@ -104,10 +104,10 @@ Section typing.
   Context `{typeG Σ}.
 
   Lemma tctx_borrow E L p n ty κ :
-    tctx_incl E L [TCtx_holds p (own n ty)]
-                  [TCtx_holds p (&uniq{κ}ty); TCtx_guarded p κ (own n ty)].
+    tctx_incl E L [TCtx_hasty p (own n ty)]
+                  [TCtx_hasty p (&uniq{κ}ty); TCtx_guarded p κ (own n ty)].
   Proof.
-    iIntros (tid) "#LFT _ _ H".
+    iIntros (tid ??) "#LFT $ $ H".
     rewrite /tctx_interp big_sepL_singleton big_sepL_cons big_sepL_singleton.
     iDestruct "H" as (v) "[% Hown]". iDestruct "Hown" as (l) "(EQ & Hmt & ?)".
     iDestruct "EQ" as %[=->]. iMod (bor_create with "LFT Hmt") as "[Hbor Hext]". done.
@@ -119,10 +119,13 @@ Section typing.
 
   Lemma tctx_reborrow_uniq E L p ty κ κ' :
     lctx_lft_incl E L κ' κ →
-    tctx_incl E L [TCtx_holds p (&uniq{κ}ty)]
-                  [TCtx_holds p (&uniq{κ'}ty); TCtx_guarded p κ (&uniq{κ}ty)].
+    tctx_incl E L [TCtx_hasty p (&uniq{κ}ty)]
+                  [TCtx_hasty p (&uniq{κ'}ty); TCtx_guarded p κ (&uniq{κ}ty)].
   Proof.
-    iIntros (Hκκ' tid) "#LFT #HE #HL H". iDestruct (Hκκ' with "HE HL") as "Hκκ'".
+    iIntros (Hκκ' tid ??) "#LFT HE HL H".
+    iDestruct (elctx_interp_persist with "HE") as "#HE'".
+    iDestruct (llctx_interp_persist with "HL") as "#HL'". iFrame "HE HL".
+    iDestruct (Hκκ' with "HE' HL'") as "Hκκ'".
     rewrite /tctx_interp big_sepL_singleton big_sepL_cons big_sepL_singleton.
     iDestruct "H" as (v) "[% Hown]". iDestruct "Hown" as (l P) "[[EQ #Hiff] Hb]".
     iDestruct "EQ" as %[=->]. iMod (bor_iff with "LFT [] Hb") as "Hb". done. by eauto.
